Prove eval_steps_imp_steps

pancake/semantics/timeFunSemScript.sml
@@ -85,14 +85,6 @@ Definition pick_eval_output_term_def:
   (pick_eval_output_term _ [] = (NONE, NONE))
 End
 
-Definition eval_delay_def:
-  eval_delay st =
-  (LDelay 1 ,
-   st with
-      <|clocks := delay_clocks (st.clocks) 1;
-        ioAction := NONE|>)
-End
-
 
 Definition eval_delay_wtime_none_def:
   eval_delay_wtime_none st m n =
@@ -102,6 +94,19 @@ Definition eval_delay_wtime_none_def:
        (LDelay 1 ,
         st with
            <|clocks := delay_clocks (st.clocks) 1;
+             ioAction := NONE|>)
+  else NONE
+End
+
+Definition eval_delay_wtime_some_def:
+  eval_delay_wtime_some st m n w =
+  if 1 ≤ w ∧ w + n < m ∧
+     max_clocks (delay_clocks (st.clocks) (n + 1)) m
+  then SOME
+       (LDelay 1 ,
+        st with
+           <|clocks := delay_clocks (st.clocks) 1;
+             waitTime := SOME (w - 1);
              ioAction := NONE|>)
   else NONE
 End
@@ -123,7 +128,7 @@ Definition eval_output_def:
   eval_output prog m n st =
   case ALOOKUP prog st.location of
   | SOME tms =>
-      if machine_bounds (resetOutput st) m (m - n) tms
+      if n < m ∧ machine_bounds (resetOutput st) m (m - n) tms
       then (case pick_eval_output_term (resetOutput st) tms of
             | (SOME os, SOME st') => SOME (LAction (Output os), st')
             | _ => NONE)
@@ -144,9 +149,27 @@ Definition eval_step_def:
       then eval_output prog m n st
       else
         (case or orn of
-         | Delay => SOME (eval_delay st)
+         | Delay => eval_delay_wtime_some st m n w
          | Input i => eval_input prog m n i st)
 End
+
+
+Definition eval_steps_def:
+  (eval_steps (0:num) prog m n or st (lbls, sts) = SOME (lbls, sts)) ∧
+  (eval_steps (SUC k) prog m n or st (lbls, sts) =
+   case eval_step prog m n or k st of
+   | SOME (lbl, st') =>
+       let n' =
+           case lbl of
+           | LDelay d => d + n
+           | LAction _ => n
+       in
+         (case eval_steps k prog m n' or st' (lbls, sts) of
+          | NONE => NONE
+          | SOME (lbls', sts') => SOME (lbl::lbls', st'::sts'))
+   | NONE => NONE)
+End
+
 
 Theorem pick_eval_input_term_imp_pickTerm:
   ∀tms st m n i st'.
@@ -221,7 +244,68 @@ Proof
 QED
 
 
-Theorem foo:
+Theorem pick_eval_output_term_imp_pickTerm:
+  ∀tms st m n os st'.
+    machine_bounds (resetOutput st) m (m − n) tms ∧
+    pick_eval_output_term (resetOutput st) tms = (SOME os,SOME st') ⇒
+    pickTerm (resetOutput st) m (m − n) NONE tms st' ∧
+    st'.ioAction = SOME (Output os)
+Proof
+  Induct >>
+  rpt gen_tac >>
+  strip_tac >>
+  gs []
+  >- gs [pick_eval_output_term_def] >>
+  gs [pick_eval_output_term_def] >>
+  cases_on ‘h’ >> gs [] >>
+  reverse (cases_on ‘i’) >> gs []
+  >- (
+    FULL_CASE_TAC >> gs [] >> rveq >> gs []
+    >- (
+      rewrite_tac [Once pickTerm_cases] >>
+      gs [] >>
+      gs [machine_bounds_def, terms_time_range_def,
+          conds_eval_lt_dimword_def, input_terms_actions_def,
+          terms_in_signals_def] >>
+      gs [eval_term_def, evalTerm_cases] >>
+      rveq >> gs [state_component_equality]) >>
+    rewrite_tac [Once pickTerm_cases] >>
+    gs [] >>
+    last_x_assum (qspecl_then [‘st’, ‘m’, ‘n’, ‘os’, ‘st'’] mp_tac) >>
+    impl_tac
+    >- (
+      gs [] >>
+      gs [machine_bounds_def, tms_conds_eval_def, conds_eval_lt_dimword_def,
+          terms_time_range_def, input_terms_actions_def, terms_wtimes_ffi_bound_def,
+          terms_in_signals_def]) >>
+    strip_tac >>
+    gs [machine_bounds_def, terms_time_range_def,
+        conds_eval_lt_dimword_def, input_terms_actions_def,
+        terms_in_signals_def, tms_conds_eval_def,  tm_conds_eval_def,
+        timeLangTheory.termConditions_def] >>
+    gs [EVERY_MEM] >>
+    disj2_tac >>
+    rw [] >>
+    res_tac >> gs []  >>
+    FULL_CASE_TAC >> gs []) >>
+  rewrite_tac [Once pickTerm_cases] >>
+  gs [] >>
+  last_x_assum (qspecl_then [‘st’, ‘m’, ‘n’, ‘os’, ‘st'’] mp_tac) >>
+  impl_tac
+  >- (
+    gs [] >>
+    gs [machine_bounds_def, tms_conds_eval_def, conds_eval_lt_dimword_def,
+        terms_time_range_def, input_terms_actions_def, terms_wtimes_ffi_bound_def,
+        terms_in_signals_def]) >>
+  strip_tac >>
+  gs [machine_bounds_def, terms_time_range_def,
+      conds_eval_lt_dimword_def, input_terms_actions_def,
+      terms_in_signals_def, tms_conds_eval_def,  tm_conds_eval_def,
+      timeLangTheory.termConditions_def]
+QED
+
+
+Theorem eval_step_imp_step:
   eval_step prog m n or orn st = SOME (label, st') ⇒
   step prog label m n st st'
 Proof
@@ -242,51 +326,50 @@ Proof
     imp_res_tac pick_eval_input_term_imp_pickTerm >>
     gs [step_cases, mkState_def])
   >- (
+    FULL_CASE_TAC >> gs []
+    >- (
+      gs [eval_output_def] >>
+      every_case_tac >> rveq >> gs [] >>
+      rveq >> gs [] >>
+      qmatch_asmsub_rename_tac ‘ALOOKUP _ _ = SOME tms’ >>
+      imp_res_tac pick_eval_output_term_imp_pickTerm >>
+      gs [step_cases, mkState_def]) >>
+    gs [eval_delay_wtime_some_def] >>
+    rveq >>
+    gs [step_cases, mkState_def] >>
+    gs [state_component_equality]) >>
   FULL_CASE_TAC >> gs []
   >- (
     gs [eval_output_def] >>
     every_case_tac >> rveq >> gs [] >>
     rveq >> gs [] >>
     qmatch_asmsub_rename_tac ‘ALOOKUP _ _ = SOME tms’ >>
-
-
-
-    )
-
-
-
-
-
-  )
-
-
-
-
-
-
-    metis_tac [pick_eval_input_term_imp_pickTerm]
-
-
-
-
-
-
-  )
-
-
-
-
-
+    imp_res_tac pick_eval_output_term_imp_pickTerm >>
+    gs [step_cases, mkState_def]) >>
+  gs [eval_input_def] >>
+  FULL_CASE_TAC >> gs [] >>
+  FULL_CASE_TAC >> gs [] >> rveq >> gs [] >>
+  qmatch_asmsub_rename_tac ‘ALOOKUP _ _ = SOME tms’ >>
+  imp_res_tac pick_eval_input_term_imp_pickTerm >>
+  gs [step_cases, mkState_def]
 QED
 
 
+Theorem eval_steps_imp_steps:
+  ∀k prog m n or st labels sts.
+    eval_steps k prog m n or st ([],[]) = SOME (labels, sts) ⇒
+    steps prog labels m n st sts
+Proof
+  Induct >> rw []
+  >- fs [eval_steps_def, steps_def] >>
+  gs [eval_steps_def] >>
+  every_case_tac >> gs [] >> rveq >> gs [] >>
+  gs [steps_def] >>
+  imp_res_tac eval_step_imp_step >>
+  gs [] >>
+  res_tac >> gs []
+QED
 
-
-
-(*
- step_eval s or = SOME (s',label) ==>
-  step label s s'
-*)
 
 
 (*
